Refactoring of the copy-mac security proofs

casestudy/copy_mac_cache_ct_proof.ec
@@ -3,24 +3,8 @@ from Jasmin require import JModel.
 
 require import Array128 WArray128.
 
-require Copy_mac_ct_proof.
-
-theory LeakageModelCL.
-
-op leak_div_32 (a b: W32.t) : address list = [].
-
-op leak_div_64 (a b: W64.t) : address list = [].
-
-op leak_mem (a: address) : address =
-  a %/ 64.
-
-end LeakageModelCL.
-
-theory LeakageModelTVCL.
-  op leak_div_32 = Copy_mac_ct_proof.LeakageModelTV.leak_div_32.
-  op leak_div_64 = Copy_mac_ct_proof.LeakageModelTV.leak_div_64.
-  op leak_mem = LeakageModelCL.leak_mem.
-end LeakageModelTVCL.
+require Copy_mac_ct.
+require import Leakage_models.
 
 clone import Copy_mac_ct.T with
 theory LeakageModel <- LeakageModelTVCL.
@@ -33,7 +17,7 @@ equiv l_rotate_offset_div md_size_ : M.rotate_offset_div ~ M.rotate_offset_div:
 ==> ={M.leakages} /\ 0 <= to_uint res{1} < to_uint md_size_ /\ 0 <= to_uint res{2} < to_uint md_size_.
 proof.
   proc; wp; skip => /> *.
-  rewrite /leak_div_32 !Copy_mac_ct_proof.l_rotate_offset_div_core //.
+  rewrite /leak_div_32 !l_rotate_offset_div_core //.
   smt (W32.to_uint_small W32.to_uint_cmp).
 qed.
 
